---
title: "Year 9 Maths Chapter 2 - Expressions, equations and inequalities"
layout: default
parent: Year 9 Maths
nav_order: 3
---

# Year 9 Maths Chapter 2 - Expressions, equations and inequalities
{: .no_toc }

<label class="label label-blue">In-Progress</label>

*You will want to refer to [Year 7 Maths Chapter 9](../y7/y7c10.html) and [Year 8 Maths Chapter 2](../y8/y8c2.html) for basic equations. This section is more advanced, and omits basic concepts.*

#### Table of Contents
{: .no_toc }

* Table of Contents
{:toc}

***


## Inequalities

- Similar to an equation
- Always give answer in terms of the pronumeral.
- When dividing by a negative, reverse the inequality sign


#### EXAMPLE
```
4 - 5x < 1
-5 x < -3
5x > 3 # we divide by -1, and reverse the inequality sign accordingly
x > â…—
```

### Inequalities on a number line

- Open circle for `>` (greater than) and `<` (less than). For example: `x > 1` = x is greater than 1
- Closed circle for `â‰¥` (greater than or equal to) and `â‰¤` (less than or equal to). For example: `x â‰¤ 1` = x is less than or equal to 1
- Representing sets on a number line (e.g `-2 < x â‰¤ 3`) can be done like this:

![Inequalities](/resources/maths/inequalites1.jpg)

**The arrow on the number line points the same direction as the sign**

***

## Simulataneous Equations
**it makes me want to eliminate... eliminate YOU!**

You can solve simultaneous equations in different ways, graphically, using substitution, and using elimination. We will only cover substitution and elimination here.

### Substitution

Substitute one equation into the other, and solve.

#### Example
    y = 2x - 4 [1]
    4x - y = 6 [2]

    Sub [1] -> [2]

    4x - (2x - 4) = 6
    4x - 2x + 4 = 6
    2x + 4 = 6
    2x = 2
    x = 1

### Elimination

You can add or subtract equations together to eliminate pronumerals. 

- Decide whether you should add or subtract.
- If you can't add or subtract, multiply the equations to get a common pronumeral (similar to fractions)
- Eliminate the pronumeral and solve

#### Example
    3x - y = 4 [1]
    5x + y = 4 [2]

    # add the equations together

    3x + 5x + (-y) + y = 8
    8x = 8
    Therefore, x = 1

What if it isn't possible to eliminate a pronumeral in the equations' current form?

#### Example
    7x - 2y = 3 [1]
    4x - 5y = 6 [2]

    # multiply [1] by 4 and [2] by 7

    28x - 8y = 12 [1]
    28x - 35y = -42 [2]

    # [1] - [2]

    -8y - 35y = 12 - (-42)
    -43y = 54

