---
title: "Year 9 Maths Chapter 4 – Linear Relationships"
layout: default
parent: "Year 9 Maths"
nav_order: 5
---

# Year 9 Maths Chapter 4 – Linear Relationships
{: .no_toc }

<label class="label label-green">Complete</label>

*You will want to refer to [Year 8 Maths Chapter 7](../y8/y8c7.html) for basic linear relationships. This section is more advanced, and omits basic concepts.*

#### Table of Contents
{: .no_toc }

* Table of Contents
{:toc}

***

## Intercepts

x-intercept = `y = 0`
y-intercept = `x = 0`
***

## Gradient

The gradient is a measure of slope.

```
            rise
Gradient = ––––––
            run
```
***

Be careful when the gradient is negative.

## Gradient-intercept form

```
y = mx + b
```

where `m` is the gradient, and `b` is the y-intercept.
***

## General Form

```
ax + by = c
```
or
```
ax + by + c = 0
```

where a, b and c are constants. It is typically the result of an expanded FOIL.
***

## Midpoints

The midpoint is the halfway point between two end points. To find the midpoint, use the midpoint formula.
```
    ┌ x1 + x2   y1 + y2 ┐
M = | ––––––– , ––––––– |
    └    2         2    ┘
```

The `x` coordinate is the average of the two `x` coordinates
The `y` coordinate is the average of the two `y` coordinates

## Distance formula

To find a length of a line, use [Pythag](../y8/y8c3.html#pythag).

Alternatively, use the Distance Formula.

```
     ___________________________
d = √ (x2 - x1)^2 + (y2 - y1)^2 
```

#### Example

```
     _______________________________
d = √ ((-7) - (-3))^2 + ((-4)-2)^2
     _________________
d = √ (-4)^2 + (-6)^2

d = √52
d = 2√13
d = 7.21 units (2dp)
```

## Direct proportion/direct variance

If b is directly proportional to a:

```
b = ka
```

where k is a constant.

Also known as:
```
y = mx
```

## Parallel lines and perpendicular lines:

If two lines are parallel they have the same gradient.
If two lines are perpendicular (at right angles) then they are reciprocals of each other.

```
Let the gradients of two perpendicular lines be m1 and m2.

m1 x m2 = -1
      1
m2 = –––
      m1

Hence, m2 is equal to the reciprocal of m1
```



